io/IIO.fst
@@ -4,11 +4,9 @@ open FStar.Tactics
 open ExtraTactics
 open FStar.Calc
 
-open Common
-open DMFree
 open IO.Sig
 open IO.Sig.Call
-open IO
+open DMFree
 
 (** The postcondition for an io computation is defined over the
 result (type: a) and local trace (type: trace).
@@ -23,17 +21,17 @@ At the end of an io computation, the local trace is appended
 in reverse order to the history. **)
 let dm_iio_theta #a = theta #a #iio_cmds #iio_sig #event iio_wps
   
-let dm_iio = dm iio_cmds iio_sig event iio_wps
+type dm_iio = dm iio_cmds iio_sig event iio_wps
 let dm_iio_return (a:Type) (x:a) : dm_iio a (hist_return x) =
   dm_return iio_cmds iio_sig event iio_wps a x
 
 val dm_iio_bind  : 
   a: Type ->
   b: Type ->
-  wp_v: Hist.hist a ->
-  wp_f: (_: a -> Prims.Tot (Hist.hist b)) ->
+  wp_v: hist a ->
+  wp_f: (_: a -> hist b) ->
   v: dm_iio a wp_v ->
-  f: (x: a -> Prims.Tot (dm_iio b (wp_f x))) ->
+  f: (x: a -> dm_iio b (wp_f x)) ->
   Tot (dm_iio b (hist_bind wp_v wp_f))
 let dm_iio_bind a b wp_v wp_f v f = dm_bind iio_cmds iio_sig event iio_wps a b wp_v wp_f v f
 
@@ -47,18 +45,22 @@ let dm_iio_subcomp a wp1 wp2 f = dm_subcomp iio_cmds iio_sig event iio_wps a wp1
 
 let dm_iio_if_then_else a wp1 wp2 f g b = dm_if_then_else iio_cmds iio_sig event iio_wps a wp1 wp2 f g b
 
+#set-options "--print_universes"
+
 val lift_pure_dm_iio :
-  a: Type ->
+  a: Type u#a ->
   w: pure_wp a ->
-  f: (_: eqtype_as_type unit -> Prims.PURE a w) ->
+  f: (eqtype_as_type unit -> PURE a w) ->
   Tot (dm_iio a (wp_lift_pure_hist w))
-let lift_pure_dm_iio a w f = lift_pure_dm iio_cmds iio_sig event iio_wps a w f
+let lift_pure_dm_iio = lift_pure_dm iio_cmds iio_sig event iio_wps
 
 
+[@@allow_informative_binders]
 total
+reifiable
 reflectable
 effect {
-  IIOwp (a:Type) (wp : hist a) 
+  IIOwp (a:Type) (wp : hist #event a) 
   with {
        repr       = dm_iio
      ; return     = dm_iio_return
@@ -68,7 +70,7 @@ effect {
      }
 }
 
-assume val __reify_IIOwp (#a:Type) (#wp:Hist.hist a) ($f:unit -> IIO.IIOwp a wp) : IIO.dm_iio a wp
+sub_effect PURE ~> IIOwp = lift_pure_dm_iio
 
 effect IIO
   (a:Type)
@@ -76,98 +78,5 @@ effect IIO
   (post : trace -> a -> trace -> Type0) =
   IIOwp a (to_hist pre post) 
 
-sub_effect PURE ~> IIOwp = lift_pure_dm_iio
-
-(** This is a identity function, and we need it because
-F* does not have depth subtyping on inductives. **)
-let rec cast_io_iio #a (x:io a) : iio a =
-  match x with
-  | Return z -> Return z
-  | Call (cmd:io_cmds) args fnc ->
-     Call cmd args (fun res -> cast_io_iio (fnc res))
-  | PartialCall pre fnc ->
-     PartialCall pre (fun res -> cast_io_iio (fnc res))
-
-let rec lemma_cast_io_iio #a (m:io a) :
-  Lemma
-    (dm_io_theta m `hist_ord` dm_iio_theta (cast_io_iio m)) = 
-  match m with
-  | Return _ -> ()
-  | PartialCall pre k ->begin
-    let fst : squash pre -> hist a = fun r -> dm_io_theta (k r) in
-    let snd : squash pre -> hist a = fun r -> dm_iio_theta (cast_io_iio (k r)) in
-    calc (==) {
-      dm_io_theta m;
-      == {}
-      dm_io_theta (PartialCall pre k);
-      == { _ by (norm [delta_only [`%dm_io_theta;`%theta]; zeta; iota]) } // unfold theta
-      hist_bind (partial_call_wp pre) (fun r -> dm_io_theta (k r));
-      == {}
-      hist_bind (partial_call_wp pre) fst;
-    };
-    (** fst ==> snd /\ hist is monotonic **)
-    introduce forall (p:hist_post a) h. hist_bind (partial_call_wp pre) fst p h ==> hist_bind (partial_call_wp pre) snd p h with begin 
-      introduce forall (r:squash pre). (fst r `hist_ord` snd r) with begin
-        lemma_cast_io_iio (k r)
-      end
-    end;
-    calc (==) {
-      hist_bind (partial_call_wp pre) snd;
-      == {}
-      hist_bind (partial_call_wp pre) (fun r -> dm_iio_theta (cast_io_iio (k r)));
-      == { _ by (norm [delta_only [`%dm_iio_theta;`%theta]; zeta; iota]) }
-      dm_iio_theta (PartialCall pre (fun r -> cast_io_iio (k r)));
-      == { _ by (compute ()) }
-      dm_iio_theta (cast_io_iio (PartialCall pre k));
-      == {}
-      dm_iio_theta (cast_io_iio m);
-    }
-  end
-  | Call (cmd:io_cmds) arg k -> begin
-    let fst : io_sig.res cmd arg -> hist a = fun r -> dm_io_theta (k r) in
-    let snd : iio_sig.res cmd arg -> hist a = fun r -> dm_iio_theta (cast_io_iio (k r)) in
-    calc (==) {
-      dm_io_theta m;
-      == {}
-      dm_io_theta (Call cmd arg k);
-      == { _ by (norm [delta_only [`%dm_io_theta;`%theta]; zeta; iota]) } // unfold theta
-      hist_bind (iio_wps cmd arg) (fun r -> dm_io_theta (k r));
-      == {}
-      hist_bind (iio_wps cmd arg) fst;
-    };
-    (** fst ==> snd /\ hist is monotonic **)
-    introduce forall (p:hist_post a) h. hist_bind (iio_wps cmd arg) fst p h ==> hist_bind (iio_wps cmd arg) snd p h with begin 
-      introduce forall (r:iio_sig.res cmd arg). (fst r `hist_ord` snd r) with begin
-        lemma_cast_io_iio (k r)
-      end
-    end;
-    calc (==) {
-      hist_bind (iio_wps cmd arg) snd;
-      == {}
-      hist_bind (iio_wps cmd arg) (fun r -> dm_iio_theta (cast_io_iio (k r)));
-      == { _ by (norm [delta_only [`%dm_iio_theta;`%theta]; zeta; iota]) }
-      dm_iio_theta (Call cmd arg (fun r -> cast_io_iio (k r)));
-      == { _ by (compute ()) }
-      dm_iio_theta (cast_io_iio (Call cmd arg k));
-      == {}
-      dm_iio_theta (cast_io_iio m);
-    }
-  end
-
-let lemma_cast_io_iio_2 #a (x:io a) (wp:hist a) :
-  Lemma
-    (requires (wp `hist_ord` dm_io_theta x))
-    (ensures (wp `hist_ord` dm_iio_theta (cast_io_iio x))) =
-  lemma_cast_io_iio x
-
-let lift_io_iio (a:Type) (wp:hist a) (f:dm_io a wp) :
-  Tot (dm_iio a wp) =
-  lemma_cast_io_iio_2 f wp;
-  cast_io_iio f
-
-sub_effect IOwp ~> IIOwp = lift_io_iio
-
-
-let get_trace () : IIOwp trace
-  (fun p h -> forall lt. lt == [] ==> p lt h) =
+let get_trace () : IIOwp trace (fun p h -> forall lt. lt == [] ==> p lt h) =
   IIOwp?.reflect (iio_call GetTrace ())
