io/TC.Monitorable.Hist.fst
@@ -3,9 +3,7 @@ module TC.Monitorable.Hist
 open FStar.Tactics
 open FStar.Tactics.Typeclasses
 
-open Common
 open IO.Sig 
-open Hist
 
 type monitorable_prop = (cmd:io_cmds) -> (io_sig.args cmd) -> (history:trace) -> Tot bool
 
@@ -26,7 +24,7 @@ let rec enforced_locally
     if has_event_respected_pi e check h then enforced_locally (check) (e::h) t
     else false
   
-unfold let pi_as_hist (#a:Type) (pi:monitorable_prop) : hist a =
+let pi_as_hist (#a:Type) (pi:monitorable_prop) : hist a =
   (fun p h -> forall r lt. enforced_locally pi h lt ==> p lt r)
 
 let lemma_bind_pi_implies_pi (#a #b:Type) (pi:monitorable_prop) : 
